scratch/State_Heap.thy
@@ -27,7 +27,7 @@ lemma lift_p_P:
   "case the (execute f heap) of (_, heap) \<Rightarrow> P heap"
   using execute_cases by (auto split: option.split_asm)
 
-lemma lift_p_P'[intro]:
+lemma lift_p_P':
   "P heap'" if "the (execute f heap) = (v, heap')"
   using that lift_p_P by auto
 
@@ -35,14 +35,17 @@ lemma lift_p_the_Some[simp]:
   "execute f heap = Some (v, heap')" if "the (execute f heap) = (v, heap')"
   using that execute_cases by (auto split: option.split_asm)
 
+lemma lift_p_E:
+  obtains v heap' where "execute f heap = Some (v, heap')" "P heap'"
+  using execute_cases by (cases "execute f heap") auto
+
 end
 
-context
+locale heap_mem =
   fixes P :: "heap \<Rightarrow> bool"
-    and lookup :: "heap \<Rightarrow> 'k \<Rightarrow> 'v option"
-    (* and lookup :: "'k \<Rightarrow> 'v option Heap" *)
-    and update :: "'k \<Rightarrow> 'v \<Rightarrow> 'something Heap"
-  (* assumes lookup_inv: "lift_p P (lookup k)" *)
+    and lookup :: "'k \<Rightarrow> 'v option Heap"
+    and update :: "'k \<Rightarrow> 'v \<Rightarrow> unit Heap"
+  assumes lookup_inv: "lift_p P (lookup k)"
   assumes update_inv: "lift_p P (update k v)"
 begin
 
@@ -52,23 +55,29 @@ definition rel_state :: "('a \<Rightarrow> 'b \<Rightarrow> bool) \<Rightarrow> 
       (case runState f heap of (v1, heap1) \<Rightarrow> case execute g heap of
         Some (v2, heap2) \<Rightarrow> R v1 v2 \<and> heap1 = heap2 \<and> P heap2 | None \<Rightarrow> False)"
 
-definition "lookup1 k \<equiv> State (\<lambda> heap. (lookup heap k, heap))"
+definition "lookup' k \<equiv> State (\<lambda> heap. the (execute (lookup k) heap))"
 
-definition "lookup2 k \<equiv> Heap_Monad.Heap (\<lambda> heap. Some (lookup heap k, heap))"
+lemma rel_state_lookup:
+  "rel_state (op =) (lookup' k) (lookup k)"
+  unfolding rel_state_def lookup'_def using lookup_inv[of k] by (auto intro: lift_p_P')
 
 definition "update' k v \<equiv> State (\<lambda> heap. the (execute (update k v) heap))"
 
 lemma rel_state_update:
   "rel_state (op =) (update' k v) (update k v)"
-  unfolding rel_state_def update'_def using update_inv[of k v] by auto
-
-lemma
-  "rel_state (op =) (lookup1 k) (lookup2 k)"
-  unfolding rel_state_def lookup1_def lookup2_def by auto
+  unfolding rel_state_def update'_def using update_inv[of k v] by (auto intro: lift_p_P')
 
 context
   includes lifting_syntax
 begin
+
+lemma transfer_lookup:
+  "(op = ===> rel_state (op =)) lookup' lookup"
+  unfolding rel_fun_def by (auto intro: rel_state_lookup)
+
+lemma transfer_update:
+  "(op = ===> op = ===> rel_state (op =)) update' update"
+  unfolding rel_fun_def by (auto intro: rel_state_update)
 
 lemma rel_state_elim:
   assumes "rel_state R f g" "P heap"
@@ -118,8 +127,8 @@ lemma transfer_get[transfer_rule]:
 
 definition checkmem_heap :: "'k \<Rightarrow> 'v Heap \<Rightarrow> 'v Heap" where
   "checkmem_heap param calc \<equiv>
-    Heap_Monad.bind heap_get (\<lambda> M.
-    case lookup M param of
+    Heap_Monad.bind (lookup param) (\<lambda> x.
+    case x of
       Some x \<Rightarrow> return x
     | None \<Rightarrow> Heap_Monad.bind calc (\<lambda> x.
         Heap_Monad.bind (update param x) (\<lambda> _.
@@ -129,42 +138,268 @@ definition checkmem_heap :: "'k \<Rightarrow> 'v Heap \<Rightarrow> 'v Heap" whe
   )
   "
 
-lemma
+lemma transfer_checkmem_heap:
   "(op = ===> rel_state op = ===> rel_state op =)
-    (mem_defs.checkmem lookup (\<lambda> heap k v. snd (the (execute (update k v) heap)))) checkmem_heap"
-  unfolding mem_defs.checkmem_def checkmem_heap_def
+    (mem_defs.checkmem lookup' update') checkmem_heap"
+  supply [transfer_rule] = transfer_lookup transfer_update
+  unfolding mem_defs.checkmem_def checkmem_heap_def by transfer_prover
 
-  unfolding rel_fun_def
+definition map_of_heap where
+  "map_of_heap heap k = fst (the (execute (lookup k) heap))"
+
+context
+  assumes
+    lookup_correct: "map_of_heap (snd (the (execute (lookup k) m))) \<subseteq>\<^sub>m (map_of_heap m)"
+      and
+    update_correct: "map_of_heap (snd (the (execute (update k v) m))) \<subseteq>\<^sub>m (map_of_heap m)(k \<mapsto> v)"
+begin
+
+lemma lookup'_correct:
+  "mem_defs.map_of lookup' (snd (runState (lookup' k) m)) \<subseteq>\<^sub>m (mem_defs.map_of lookup' m)"
+  unfolding mem_defs.map_of_def map_le_def lookup'_def
   apply auto
-  apply (rule transfer_bind[unfolded rel_fun_def, rule_format])
-   apply (rule transfer_get[unfolded rel_fun_def, rule_format])
-  apply (rule option.case_transfer[unfolded rel_fun_def, rule_format, where R = "op ="])
-  subgoal for x xa y xb ya
-    unfolding Monad.bind_def Heap_Monad.bind_def Monad.get_def Heap_Monad.return_def return_def
-    apply (auto split: option.splits)
-    apply (rule rel_state_intro)
-     apply (auto split: option.splits)
-       apply (auto elim: rel_state_elim; fail)
-      apply (erule rel_state_elim)
-       apply assumption
-      apply (auto split: prod.split_asm)[]
-    using lift_p_None[OF update_inv[of x]]
-      apply blast
-     apply (auto split: prod.split_asm simp: execute_heap Monad.return_def put_def)[]
-      apply (force elim: rel_state_elim)
-     apply (force elim: rel_state_elim)
-    apply (auto split: prod.split_asm simp: execute_heap Monad.return_def put_def)[]
-    subgoal for heap v x2
-      apply (auto 4 4 split: option.split_asm dest: execute_cases[OF update_inv, of _ x v] elim: rel_state_elim)
-      done
-    done
-  subgoal
-    apply (rule transfer_return[unfolded rel_fun_def, rule_format])
-    by simp
-  subgoal
-    by (auto intro: option.rel_refl)
+  by (metis (mono_tags, lifting) domIff lookup_correct map_le_def map_of_heap_def option.simps(3))
+
+lemma update'_correct:
+  "mem_defs.map_of lookup' (snd (runState (update' k v) m)) \<subseteq>\<^sub>m mem_defs.map_of lookup' m(k \<mapsto> v)"
+  unfolding mem_defs.map_of_def map_le_def lookup'_def update'_def
+  apply auto
+   apply (smt domIff fun_upd_apply map_le_def map_of_heap_def option.simps(1) option.simps(3) update_correct)
+  apply (smt domIff fun_upd_apply map_le_def map_of_heap_def option.simps(1) option.simps(3) update_correct)
   done
 
-end
+lemma lookup'_inv:
+  "DP_CRelVS.lift_p P (lookup' k)"
+  unfolding DP_CRelVS.lift_p_def lookup'_def by (auto elim: lift_p_P'[OF lookup_inv])
 
-end
+lemma update'_inv:
+  "DP_CRelVS.lift_p P (update' k v)"
+  unfolding DP_CRelVS.lift_p_def update'_def by (auto elim: lift_p_P'[OF update_inv])
+
+interpretation state: mem_correct lookup' update' P
+  by (intro mem_correct.intro lookup'_correct update'_correct lookup'_inv update'_inv)
+
+context
+  fixes dp :: "'k \<Rightarrow> 'v"
+begin
+
+interpretation dp_consistency lookup' update' P dp ..
+
+print_statement crel_vs_def rel_state_def
+
+definition "crel_vs' R v f \<equiv>
+  \<forall>heap. P heap \<and> cmem heap \<longrightarrow>
+    (case execute f heap of None \<Rightarrow> False | Some (v', heap') \<Rightarrow> P heap' \<and> R v v' \<and> cmem heap')
+"
+
+definition "state_of s \<equiv> State (\<lambda> heap. the (execute s heap))"
+
+lemma crel_vs'_execute_None:
+  False if "crel_vs' R a b" "execute b heap = None" "P heap" "cmem heap"
+  using that unfolding crel_vs'_def by auto
+
+lemma crel_vs'_execute_Some:
+  assumes "crel_vs' R a b" "P heap" "cmem heap"
+  obtains x heap' where "execute b heap = Some (x, heap')" "P heap'"
+  using assms unfolding crel_vs'_def by (cases "execute b heap") auto
+
+lemma crel_vs'_executeD:
+  assumes "crel_vs' R a b" "P heap" "cmem heap"
+  obtains x heap' where "execute b heap = Some (x, heap')" "P heap'" "cmem heap'" "R a x"
+  using assms unfolding crel_vs'_def by (cases "execute b heap") auto
+
+lemma crel_vs_state_of:
+  "crel_vs R a (state_of b)" if "crel_vs' R a b"
+  unfolding crel_vs_def state_of_def by (auto elim: crel_vs'_executeD[OF that])
+
+lemma crel_vs'I: "crel_vs' R a b" if "(crel_vs R OO rel_state (op =)) a b"
+  using that by (auto 4 3 elim: crel_vs_elim rel_state_elim simp: crel_vs'_def)
+
+lemma rel_fun_comp:
+  assumes "(R1 ===> S1) f g" "(R2 ===> S2) g h"
+  shows "(R1 OO R2 ===> S1 OO S2) f h"
+  using assms by (auto intro!: rel_funI dest!: rel_funD)
+
+lemma rel_fun_comp1:
+  assumes "(R1 ===> S1) f g" "(R2 ===> S2) g h" "R' = R1 OO R2"
+  shows "(R' ===> S1 OO S2) f h"
+  using assms rel_fun_comp by metis
+
+lemma rel_fun_comp2:
+  assumes "(R1 ===> S1) f g" "(R2 ===> S2) g h" "S' = S1 OO S2"
+  shows "(R1 OO R2 ===> S') f h"
+  using assms rel_fun_comp by metis
+
+lemma transfer'_return:
+  "(R ===> crel_vs' R) (\<lambda> x. x) return"
+proof -
+  have "(R ===> (crel_vs R OO rel_state (op =))) (\<lambda> x. x) return"
+    by (rule rel_fun_comp1 return_transfer transfer_return)+ auto
+  then show ?thesis
+    by (blast intro: rel_fun_mono crel_vs'I)
+qed
+
+lemma crel_vs_return:
+  "\<lbrakk>R x y\<rbrakk> \<Longrightarrow> crel_vs' R x (return y)"
+  by (rule transfer'_return[unfolded rel_fun_def, rule_format])
+term 0 (**)
+
+lemma bind_transfer[transfer_rule]:
+  "(crel_vs' R0 ===> (R0 ===> crel_vs' R1) ===> crel_vs' R1) (\<lambda>v f. f v) (op \<bind>)"
+  unfolding rel_fun_def bind_def
+  by safe (subst crel_vs'_def, auto 4 4 elim: crel_vs'_execute_Some elim!: crel_vs'_executeD)
+
+lemma crel_vs'_update:
+  "crel_vs' op = () (update param (dp param))"
+  by (rule crel_vs'I relcomppI crel_vs_update rel_state_update)+
+
+lemma crel_vs'_lookup:
+  "crel_vs'
+    (\<lambda> v v'. case v' of None \<Rightarrow> True | Some v' \<Rightarrow> v = v' \<and> v = dp param) (dp param) (lookup param)"
+  by (rule crel_vs'I relcomppI crel_vs_lookup rel_state_lookup)+
+
+lemma crel_vs'_eq_eq_onp:
+  "crel_vs' (eq_onp (\<lambda> x. x = v)) v s" if "crel_vs' op = v s"
+  using that unfolding crel_vs'_def by (auto split: option.split simp: eq_onp_def)
+
+lemma crel_vs_bind_eq:
+  "\<lbrakk>crel_vs' op = v s; crel_vs' R (f v) (sf v)\<rbrakk> \<Longrightarrow> crel_vs' R (f v) (s \<bind> sf)"
+  by (erule bind_transfer[unfolded rel_fun_def, rule_format, OF crel_vs'_eq_eq_onp])
+     (auto simp: eq_onp_def)
+
+lemma crel_vs'_checkmem:
+  "crel_vs' op = (dp param) (checkmem_heap param s)" if "crel_vs' op = (dp param) s"
+  unfolding checkmem_heap_def
+  by (rule bind_transfer[unfolded rel_fun_def, rule_format, OF crel_vs'_lookup])
+     (auto 4 3 split: option.split_asm intro: crel_vs_bind_eq crel_vs'_update crel_vs_return that)
+
+lemma transfer_fun_app_lifted[transfer_rule]:
+  "(crel_vs' (R0 ===> crel_vs' R1) ===> crel_vs' R0 ===> crel_vs' R1)
+    (\<lambda> f x. f x) (\<lambda> f\<^sub>T' x\<^sub>T'. f\<^sub>T' \<bind> (\<lambda> f. x\<^sub>T' \<bind> (\<lambda> x. f x)))"
+  unfolding fun_app_lifted_def by transfer_prover
+
+end (* Dynamic Programming Problem *)
+
+context
+  fixes dp :: "'k \<Rightarrow> 'v"
+begin
+
+interpretation dp_consistency lookup' update' P dp ..
+
+definition "crel_vs1 R v f \<equiv>
+  \<forall>heap. P heap \<longrightarrow>
+    (case execute f heap of None \<Rightarrow> False | Some (v', heap') \<Rightarrow> P heap' \<and> (cmem heap \<longrightarrow> R v v' \<and> cmem heap'))
+"
+
+lemma crel_vs1_execute_None:
+  False if "crel_vs1 R a b" "execute b heap = None" "P heap"
+  using that unfolding crel_vs1_def by auto
+
+lemma crel_vs1_execute_Some:
+  assumes "crel_vs1 R a b" "P heap"
+  obtains x heap' where "execute b heap = Some (x, heap')" "P heap'"
+  using assms unfolding crel_vs1_def by (cases "execute b heap") auto
+
+lemma crel_vs1_executeD:
+  assumes "crel_vs1 R a b" "P heap" "cmem heap"
+  obtains x heap' where "execute b heap = Some (x, heap')" "P heap'" "cmem heap'" "R a x"
+  using assms unfolding crel_vs1_def by (cases "execute b heap") auto
+
+lemma rel_state_state_of:
+  "rel_state op = (state_of b) b" if "crel_vs1 R a b"
+  unfolding rel_state_def state_of_def
+  by (auto split: option.split elim: crel_vs1_execute_Some[OF that])
+
+lemma crel_vs1_state_of:
+  "crel_vs R a (state_of b)" if "crel_vs1 R a b"
+  unfolding crel_vs_def state_of_def by (auto elim: crel_vs1_executeD[OF that])
+
+lemma crel_vs1_alt_def:
+  "crel_vs1 R = (crel_vs R OO rel_state (op =))"
+proof (intro ext)
+  fix a b
+  have "(crel_vs R OO rel_state (op =)) a b" if "crel_vs1 R a b"
+    using that by - (rule relcomppI; erule crel_vs1_state_of rel_state_state_of)
+  moreover have "crel_vs1 R a b" if "(crel_vs R OO rel_state (op =)) a b"
+    using that by (auto 4 3 elim: crel_vs_elim rel_state_elim simp: crel_vs1_def)
+  ultimately show "crel_vs1 R a b = (crel_vs R OO rel_state (op =)) a b" ..
+qed
+
+lemma transfer_return1:
+  "(R ===> crel_vs1 R) (\<lambda> x. x) return"
+  unfolding crel_vs1_alt_def by (rule rel_fun_comp1 return_transfer transfer_return)+ auto
+
+lemma crel_vs_return1:
+  "\<lbrakk>R x y\<rbrakk> \<Longrightarrow> crel_vs1 R x (return y)"
+  by (rule transfer_return1[unfolded rel_fun_def, rule_format])
+term 0 (**)
+
+lemma rel_fun_relcompp:
+  "((R1 ===> S1) OO (R2 ===> S2)) a b \<Longrightarrow> ((R1 OO R2) ===> (S1 OO S2)) a b"
+  unfolding OO_def rel_fun_def by blast
+
+lemma rel_fun_comp1':
+  assumes "(R1 ===> S1) f g" "(R2 ===> S2) g h" "\<And> a b. R' a b \<Longrightarrow> (R1 OO R2) a b"
+  shows "(R' ===> S1 OO S2) f h"
+  by (auto intro: assms rel_fun_mono[OF rel_fun_comp1])
+
+lemma rel_fun_comp2':
+  assumes "(R1 ===> S1) f g" "(R2 ===> S2) g h" "\<And> a b. (S1 OO S2) a b \<Longrightarrow> S' a b"
+  shows "(R1 OO R2 ===> S') f h"
+  by (auto intro: assms rel_fun_mono[OF rel_fun_comp1])
+
+lemma crel_vs_rel_state:
+  "(R0 ===> crel_vs R1) x (state_of o y)" if "(R0 ===> crel_vs R1 OO rel_state op =) x y"
+  using that
+  unfolding state_of_def
+  apply -
+  apply (rule rel_funI)
+  apply (drule rel_funD, assumption)
+  apply (erule relcomppE)
+  apply auto
+  apply (rule crel_vs_intro)
+  apply auto
+   apply (erule rel_state_elim, assumption)
+    apply (erule crel_vs_elim)
+      apply assumption+
+    apply simp
+  subgoal premises prems for x' y' b M v' M'
+  proof -
+    from prems(2,3) have "crel_vs1 R1 (x x') (y y')"
+      unfolding crel_vs1_alt_def by (rule relcomppI)
+    with prems show ?thesis
+      by (auto elim: crel_vs1_executeD)
+  qed
+  subgoal premises prems for x' y' b M v' M'
+  proof -
+    from prems(2,3) have "crel_vs1 R1 (x x') (y y')"
+      unfolding crel_vs1_alt_def by (rule relcomppI)
+    with prems show ?thesis
+      by (auto elim: crel_vs1_executeD)
+  qed
+  done
+
+lemma bind_transfer1:
+  "(crel_vs1 R0 ===> (R0 ===> crel_vs1 R1) ===> crel_vs1 R1) (\<lambda>v f. f v) (op \<bind>)"
+  if "\<And> x. R0 x x"
+  unfolding crel_vs1_alt_def
+  apply (rule rel_fun_comp2')
+    apply (rule bind_transfer)
+   apply (rule transfer_bind)
+  apply (drule rel_fun_relcompp)
+  apply (erule rel_fun_mono)
+   defer
+   apply assumption
+  apply (intro impI relcomppI)
+   apply (erule crel_vs_rel_state)
+  by (auto 4 4 dest: rel_funD intro: that elim: rel_state_state_of simp: crel_vs1_alt_def[symmetric])
+
+end (* Dynamic Programming Problem *)
+
+end (* Correctness *)
+
+end (* Lifting Syntax *)
+
+end (* Lookup & Update *)
+
+end (* Theory *)
